sha/spec_hmac.v
@@ -188,9 +188,9 @@ Definition hmac_relate (h: hmacabs) (r: hmacstate) : Prop :=
 
 Definition t_struct_hmac_ctx_st := Tstruct _hmac_ctx_st noattr.
 
-Definition hmacstate_ (h: hmacabs) (c: val) : mpred :=
+Definition hmacstate_ (wsh: share) (h: hmacabs) (c: val) : mpred :=
    EX r:hmacstate,
-    !!  hmac_relate h r && data_at Tsh t_struct_hmac_ctx_st r c.
+    !!  hmac_relate h r && data_at wsh t_struct_hmac_ctx_st r c.
 
 (************************ Specification of HMAC_init ********************************************)
 
@@ -208,44 +208,44 @@ Definition hmac_relate_PreInitNull (key:list Z) (h:hmacabs ) (r: hmacstate) : Pr
     innerShaInit keyB = iS /\ outerShaInit keyB = oS
   end.
 
-Definition hmacstate_PreInitNull key (h: hmacabs) (c: val) : mpred :=
+Definition hmacstate_PreInitNull (wsh: share) key (h: hmacabs) (c: val) : mpred :=
    EX r:hmacstate, EX v:_,
     !!hmac_relate_PreInitNull key h r &&
-    data_at Tsh t_struct_hmac_ctx_st
+    data_at wsh t_struct_hmac_ctx_st
        (upd_reptype t_struct_hmac_ctx_st [StructField _md_ctx] r v) c.
 
-Definition initPre (c:val) (k: val) h l key : mpred:=
+Definition initPre (wsh sh: share) (c:val) (k: val) h l key : mpred:=
   match k with
     Vint z => if Int.eq z Int.zero
-              then hmacstate_PreInitNull key h c
+              then hmacstate_PreInitNull wsh key h c
               else FF
   | Vptr b ofs => !!has_lengthK l key &&
-                  (data_at_ Tsh t_struct_hmac_ctx_st c *
-                        (data_block Tsh key (Vptr b ofs)))
+                  (data_at_ wsh t_struct_hmac_ctx_st c *
+                        (data_block sh key (Vptr b ofs)))
   | _ => FF
   end.
 
-Definition initPostKey k key:mpred :=
+Definition initPostKey (sh: share) k key:mpred :=
   match k with
     Vint z => !!(z=Int.zero) && emp
-  | Vptr b ofs => data_block Tsh key k
+  | Vptr b ofs => data_block sh key k
   | _ => FF
   end.
 
 Definition HMAC_Init_spec :=
   DECLARE _HMAC_Init
-   WITH c : val, k:val, l:Z, key:list Z, h1:hmacabs, gv:globals
+   WITH wsh: share, sh: share, c : val, k:val, l:Z, key:list Z, h1:hmacabs, gv:globals
    PRE [ _ctx OF tptr t_struct_hmac_ctx_st,
          _key OF tptr tuchar,
          _len OF tint ]
-         PROP ((*has_lengthK l key*))
+         PROP (writable_share wsh; readable_share sh (*has_lengthK l key*))
          LOCAL (temp _ctx c; temp _key k; temp _len (Vint (Int.repr l));
                 gvars gv)
-         SEP (K_vector gv; initPre c k h1 l key)
+         SEP (K_vector gv; initPre wsh sh c k h1 l key)
   POST [ tvoid ]
      PROP ()
      LOCAL ()
-     SEP (hmacstate_ (hmacInit key) c; initPostKey k key; K_vector gv).
+     SEP (hmacstate_ wsh (hmacInit key) c; initPostKey sh k key; K_vector gv).
 
 (************************ Specification of HMAC_update *******************************************************)
 
@@ -255,18 +255,19 @@ Definition has_lengthD (k l:Z) (data:list Z) :=
 
 Definition HMAC_Update_spec :=
   DECLARE _HMAC_Update
-   WITH h1: hmacabs, c : val, d:val, len:Z, data:list Z, gv: globals
+   WITH wsh:share, sh:share, h1: hmacabs, c : val, d:val, len:Z, data:list Z, gv: globals
    PRE [ _ctx OF tptr t_struct_hmac_ctx_st,
          _data OF tptr tvoid,
          _len OF tuint]
-         PROP (has_lengthD (s256a_len (absCtxt h1)) len data)
+         PROP (writable_share wsh; readable_share sh;
+                   has_lengthD (s256a_len (absCtxt h1)) len data)
          LOCAL (temp _ctx c; temp _data d; temp  _len (Vint (Int.repr len));
                 gvars gv)
-         SEP(K_vector gv; hmacstate_ h1 c; data_block Tsh data d)
+         SEP(K_vector gv; hmacstate_ wsh h1 c; data_block sh data d)
   POST [ tvoid ]
           PROP ()
           LOCAL ()
-          SEP(K_vector gv; hmacstate_ (hmacUpdate data h1) c; data_block Tsh data d).
+          SEP(K_vector gv; hmacstate_ wsh (hmacUpdate data h1) c; data_block sh data d).
 (*
 Lemma hmacUpdate_nil h x: hmac_relate h x -> hmacUpdate [] h h.
 Proof.
@@ -286,31 +287,31 @@ Definition hmac_relate_PostFinal (h:hmacabs ) (r: hmacstate) : Prop :=
     s256a_len iS = 512 /\ s256a_len oS = 512
   end.
 
-Definition hmacstate_PostFinal (h: hmacabs) (c: val) : mpred :=
+Definition hmacstate_PostFinal (wsh: share) (h: hmacabs) (c: val) : mpred :=
    EX r:hmacstate,
     !!  hmac_relate_PostFinal h r &&
-    data_at Tsh t_struct_hmac_ctx_st
+    data_at wsh t_struct_hmac_ctx_st
        (upd_reptype t_struct_hmac_ctx_st [StructField _md_ctx] r  (default_val t_struct_SHA256state_st)) c.
 
 Definition HMAC_Final_spec :=
   DECLARE _HMAC_Final
-   WITH h1: hmacabs, c : val, md:val, shmd: share, gv: globals
+   WITH wsh: share, h1: hmacabs, c : val, md:val, shmd: share, gv: globals
    PRE [ _ctx OF tptr t_struct_hmac_ctx_st,
          _md OF tptr tuchar ]
-       PROP (writable_share shmd)
+       PROP (writable_share wsh; writable_share shmd)
        LOCAL (temp _md md; temp _ctx c;
               gvars gv)
-       SEP(hmacstate_ h1 c; K_vector gv; memory_block shmd 32 md)
+       SEP(hmacstate_ wsh h1 c; K_vector gv; memory_block shmd 32 md)
   POST [ tvoid ]
           PROP ()
           LOCAL ()
-          SEP(K_vector gv; hmacstate_PostFinal (fst (hmacFinal h1)) c;
+          SEP(K_vector gv; hmacstate_PostFinal wsh (fst (hmacFinal h1)) c;
               data_block shmd (snd (hmacFinal h1)) md).
 
-Lemma hmacstate_PostFinal_PreInitNull key data dig h2 v:
+Lemma hmacstate_PostFinal_PreInitNull wsh key data dig h2 v:
       forall (Round1Final : hmacFinal (hmacUpdate data (hmacInit key)) = (h2,dig)),
-      hmacstate_PostFinal h2 v
-  |-- hmacstate_PreInitNull key h2 v.
+      hmacstate_PostFinal wsh h2 v
+  |-- hmacstate_PreInitNull wsh key h2 v.
 Proof. intros.
   unfold hmacstate_PostFinal, hmac_relate_PostFinal, hmacstate_PreInitNull; normalize.
   Exists r.
@@ -327,27 +328,27 @@ Qed.
 
 Definition HMAC_Cleanup_spec :=
   DECLARE _HMAC_cleanup
-   WITH h: hmacabs, c : val
+   WITH wsh: share, h: hmacabs, c : val
    PRE [ _ctx OF tptr t_struct_hmac_ctx_st ]
-         PROP ()
+         PROP (writable_share wsh)
          LOCAL (temp _ctx c)
-         SEP(hmacstate_PostFinal h c)
+         SEP(hmacstate_PostFinal wsh h c)
   POST [ tvoid ]
           PROP ()
           LOCAL ()
-          SEP(data_block Tsh (list_repeat (Z.to_nat(sizeof t_struct_hmac_ctx_st)) 0) c).
+          SEP(data_block wsh (list_repeat (Z.to_nat(sizeof t_struct_hmac_ctx_st)) 0) c).
 
 Definition HMAC_Cleanup_spec1 :=
   DECLARE _HMAC_cleanup
-   WITH h: hmacabs, c : val
+   WITH wsh: share, h: hmacabs, c : val
    PRE [ _ctx OF tptr t_struct_hmac_ctx_st ]
-         PROP ()
+         PROP (writable_share wsh)
          LOCAL (temp _ctx c)
-         SEP(EX key:_, hmacstate_PreInitNull key h c)
+         SEP(EX key:_, hmacstate_PreInitNull wsh key h c)
   POST [ tvoid ]
           PROP ()
           LOCAL ()
-          SEP(data_block Tsh (list_repeat (Z.to_nat(sizeof t_struct_hmac_ctx_st)) 0) c).
+          SEP(data_block wsh (list_repeat (Z.to_nat(sizeof t_struct_hmac_ctx_st)) 0) c).
 
 
 (************************ Specification of oneshot HMAC *******************************************************)
@@ -358,13 +359,13 @@ Definition HMAC_spec :=
   DECLARE _HMAC
    WITH keyVal: val, KEY:DATA,
         msgVal: val, MSG:DATA,
-        shmd: share, md: val, gv: globals
+        sh: share, shmd: share, md: val, gv: globals
    PRE [ _key OF tptr tuchar,
          _key_len OF tint,
          _d OF tptr tuchar,
          _n OF tint,
          _md OF tptr tuchar ]
-         PROP (writable_share shmd;
+         PROP (readable_share sh; writable_share shmd;
                has_lengthK (LEN KEY) (CONT KEY);
                has_lengthD 512 (LEN MSG) (CONT MSG))
          LOCAL (temp _md md; temp _key keyVal;
@@ -372,8 +373,8 @@ Definition HMAC_spec :=
                 temp _d msgVal;
                 temp _n (Vint (Int.repr (LEN MSG)));
                 gvars gv)
-         SEP(data_block Tsh (CONT KEY) keyVal;
-             data_block Tsh (CONT MSG) msgVal;
+         SEP(data_block sh (CONT KEY) keyVal;
+             data_block sh (CONT MSG) msgVal;
              K_vector gv;
              memory_block shmd 32 md)
   POST [ tptr tuchar ] EX digest:_,
@@ -381,8 +382,8 @@ Definition HMAC_spec :=
           LOCAL (temp ret_temp md)
           SEP(K_vector gv;
               data_block shmd digest md;
-              initPostKey keyVal (CONT KEY);
-              data_block Tsh (CONT MSG) msgVal).
+              initPostKey sh keyVal (CONT KEY);
+              data_block sh (CONT MSG) msgVal).
 
 (*A stronger spec of oneshot hmac that includes the cryptographic assertion in the postcondition
   is given in the verif_hmac_crpyto.v. This avoids having to Import FCF, hmacfc, and the
@@ -441,8 +442,8 @@ Ltac change_compspecs' cs cs' ::=
 
 (* TODO: maybe this lemma is not needed any more. *)
 Lemma change_compspecs_t_struct_SHA256state_st:
-  @data_at spec_sha.CompSpecs Tsh t_struct_SHA256state_st =
-  @data_at CompSpecs Tsh t_struct_SHA256state_st.
+  @data_at spec_sha.CompSpecs Ews t_struct_SHA256state_st =
+  @data_at CompSpecs Ews t_struct_SHA256state_st.
 Proof.
   extensionality gfs v.
   (* TODO: simplify this proof. *)
