mailbox/verif_mailbox_init.v
@@ -17,7 +17,7 @@ Proof.
   forward_if
   (PROP ( )
    LOCAL (temp _p p)
-   SEP (malloc_token Tsh t p * data_at_ Tsh t p)).
+   SEP (malloc_token Tsh t p * data_at_ Ews t p)).
 *
   if_tac.
     subst p. entailer!.
@@ -108,7 +108,7 @@ Proof.
          data_at_ Ews (tarray (tptr tint) N) (gv _reading); data_at_ Ews (tarray (tptr tint) N) (gv _last_read);
          EX bufs : list val, !!(Zlength bufs = i /\ Forall isptr bufs) &&
            data_at Ews (tarray (tptr tbuffer) B) (bufs ++ repeat Vundef (Z.to_nat (B - i))) (gv _bufs) *
-           fold_right sepcon emp (map (@data_at CompSpecs Tsh tbuffer (vint 0)) bufs) *
+           fold_right sepcon emp (map (@data_at CompSpecs Ews tbuffer (vint 0)) bufs) *
            fold_right sepcon emp (map (malloc_token Tsh tbuffer) bufs))).
   { unfold B, N; computable. }
   { unfold B, N; computable. }
@@ -118,7 +118,7 @@ Proof.
     { split3; simpl; auto; computable. }
     Intros b bufs.
     assert_PROP (field_compatible tint [] b) by entailer!.
-    forward_call (Tsh, tbuffer, b, 0, 1).
+    forward_call (Ews, tbuffer, b, 0, 1).
     { repeat split; simpl; auto; try computable.
       destruct H3 as [? [? [? [? ?]]]]; auto. }
     clear H3.
@@ -156,7 +156,7 @@ Proof.
            Zlength g0 = i /\ Zlength g1 = i /\ Zlength g2 = i) &&
           (data_at Ews (tarray (tptr tlock) N) (locks ++ repeat Vundef (Z.to_nat (N - i))) (gv _lock) *
            data_at Ews (tarray (tptr tint) N) (comms ++ repeat Vundef (Z.to_nat (N - i))) (gv _comm) *
-           fold_right sepcon emp (map (fun r => comm_loc Tsh (Znth r locks) (Znth r comms)
+           fold_right sepcon emp (map (fun r => comm_loc Ews (Znth r locks) (Znth r comms)
              (Znth r g) (Znth r g0) (Znth r g1) (Znth r g2) bufs
              (Znth r shs) gsh2 empty_map) (upto (Z.to_nat i))) *
            fold_right sepcon emp (map (malloc_token Tsh tlock) locks)) *
@@ -166,20 +166,20 @@ Proof.
            fold_right sepcon emp (map (malloc_token Tsh tint) comms);
          EX reads : list val, !!(Zlength reads = i) &&
            data_at Ews (tarray (tptr tint) N) (reads ++ repeat Vundef (Z.to_nat (N - i))) (gv _reading) *
-           fold_right sepcon emp (map (data_at_ Tsh tint) reads) *
+           fold_right sepcon emp (map (data_at_ Ews tint) reads) *
            fold_right sepcon emp (map (malloc_token Tsh tint) reads);
          EX lasts : list val, !!(Zlength lasts = i) &&
            data_at Ews (tarray (tptr tint) N) (lasts ++ repeat Vundef (Z.to_nat (N - i))) (gv _last_read) *
-           fold_right sepcon emp (map (data_at_ Tsh tint) lasts) *
+           fold_right sepcon emp (map (data_at_ Ews tint) lasts) *
            fold_right sepcon emp (map (malloc_token Tsh tint) lasts);
          @data_at CompSpecs Ews (tarray (tptr tbuffer) B) bufs (gv _bufs);
          EX sh : share, !!(sepalg_list.list_join sh1 (sublist i N shs) sh) &&
            @data_at CompSpecs sh tbuffer (vint 0) (Znth 0 bufs);
-         fold_right sepcon emp (map (@data_at CompSpecs Tsh tbuffer (vint 0)) (sublist 1 (Zlength bufs) bufs));
+         fold_right sepcon emp (map (@data_at CompSpecs Ews tbuffer (vint 0)) (sublist 1 (Zlength bufs) bufs));
          fold_right sepcon emp (map (malloc_token Tsh tbuffer) bufs))).
   { unfold N; computable. }
   { Exists ([] : list val) ([] : list val) ([] : list gname) ([] : list gname) ([] : list gname)
-      ([] : list gname) ([] : list val) ([] : list val) Tsh; rewrite !data_at__eq; entailer!.
+      ([] : list gname) ([] : list val) ([] : list val) Ews; rewrite !data_at__eq; entailer!.
     - rewrite sublist_same; auto; omega.
     - erewrite <- sublist_same with (al := bufs), sublist_next at 1; eauto; try (unfold B, N in *; omega).
       simpl; cancel. }
