mailbox/verif_mailbox_specs.v
@@ -32,7 +32,7 @@ Definition surely_malloc_spec :=
     POST [ tptr tvoid ] EX p:_,
        PROP ()
        LOCAL (temp ret_temp p)
-       SEP (malloc_token Tsh t p * data_at_ Tsh t p).
+       SEP (malloc_token Tsh t p * data_at_ Ews t p).
 
 Definition memset_spec :=
  DECLARE _memset
@@ -94,7 +94,7 @@ Definition initialize_channels_spec :=
  DECLARE _initialize_channels
   WITH sh1 : share, shs : list share, gv: globals
   PRE [ ]
-   PROP (Zlength shs = N; sepalg_list.list_join sh1 shs Tsh)
+   PROP (Zlength shs = N; sepalg_list.list_join sh1 shs Ews)
    LOCAL (gvars gv)
    SEP (data_at_ Ews (tarray (tptr tint) N) (gv _comm); data_at_ Ews (tarray (tptr tlock) N) (gv _lock);
         data_at_ Ews (tarray (tptr tbuffer) B) (gv _bufs);
@@ -110,7 +110,7 @@ Definition initialize_channels_spec :=
         data_at Ews (tarray (tptr tint) N) reads (gv _reading);
         data_at Ews (tarray (tptr tint) N) lasts (gv _last_read);
         fold_right sepcon emp (map (fun r =>
-          comm_loc Tsh (Znth r locks) (Znth r comms) (Znth r g) (Znth r g0)
+          comm_loc Ews (Znth r locks) (Znth r comms) (Znth r g) (Znth r g0)
             (Znth r g1) (Znth r g2) bufs (Znth r shs) gsh2 empty_map) (upto (Z.to_nat N)));
         fold_right sepcon emp (map (ghost_var gsh1 (vint 1)) g0);
         fold_right sepcon emp (map (ghost_var gsh1 (vint 0)) g1);
@@ -121,9 +121,9 @@ Definition initialize_channels_spec :=
         fold_right sepcon emp (map (malloc_token Tsh tint) reads);
         fold_right sepcon emp (map (malloc_token Tsh tint) lasts);
         data_at sh1 tbuffer (vint 0) (Znth 0 bufs);
-        fold_right sepcon emp (map (data_at Tsh tbuffer (vint 0)) (sublist 1 (Zlength bufs) bufs));
-        fold_right sepcon emp (map (data_at_ Tsh tint) reads);
-        fold_right sepcon emp (map (data_at_ Tsh tint) lasts)).
+        fold_right sepcon emp (map (data_at Ews tbuffer (vint 0)) (sublist 1 (Zlength bufs) bufs));
+        fold_right sepcon emp (map (data_at_ Ews tint) reads);
+        fold_right sepcon emp (map (data_at_ Ews tint) lasts)).
 (* All the communication channels are now inside locks. Buffer 0 also starts distributed among the channels. *)
 
 Definition initialize_reader_spec :=
@@ -133,12 +133,12 @@ Definition initialize_reader_spec :=
    PROP (readable_share sh)
    LOCAL (temp _r (vint r); gvars gv)
    SEP (data_at sh (tarray (tptr tint) N) reads (gv _reading); data_at sh (tarray (tptr tint) N) lasts (gv _last_read);
-        data_at_ Tsh tint (Znth r reads); data_at_ Tsh tint (Znth r lasts))
+        data_at_ Ews tint (Znth r reads); data_at_ Ews tint (Znth r lasts))
   POST [ tvoid ]
    PROP ()
    LOCAL ()
    SEP (data_at sh (tarray (tptr tint) N) reads (gv _reading); data_at sh (tarray (tptr tint) N) lasts (gv _last_read);
-        data_at Tsh tint Empty (Znth r reads); data_at Tsh tint (vint 1) (Znth r lasts)).
+        data_at Ews tint Empty (Znth r reads); data_at Ews tint (vint 1) (Znth r lasts)).
 
 Definition latest_read (h : hist) v :=
   (* initial condition *)
@@ -157,7 +157,7 @@ Definition start_read_spec :=
    LOCAL (temp _r (vint r); gvars gv)
    SEP (data_at sh1 (tarray (tptr tint) N) reads (gv _reading); data_at sh1 (tarray (tptr tint) N) lasts (gv _last_read);
         data_at sh1 (tarray (tptr tint) N) comms (gv _comm); data_at sh1 (tarray (tptr tlock) N) locks (gv _lock);
-        data_at_ Tsh tint (Znth r reads); data_at Tsh tint (vint b0) (Znth r lasts);
+        data_at_ Ews tint (Znth r reads); data_at Ews tint (vint b0) (Znth r lasts);
         comm_loc sh2 (Znth r locks) (Znth r comms) g g0 g1 g2 bufs sh gsh2 h;
         EX v : Z, data_at sh tbuffer (vint v) (Znth b0 bufs);
         ghost_var gsh1 (vint b0) g0)
@@ -168,7 +168,7 @@ Definition start_read_spec :=
    LOCAL (temp ret_temp (vint b))
    SEP (data_at sh1 (tarray (tptr tint) N) reads (gv _reading); data_at sh1 (tarray (tptr tint) N) lasts (gv _last_read);
         data_at sh1 (tarray (tptr tint) N) comms (gv _comm); data_at sh1 (tarray (tptr tlock) N) locks (gv _lock);
-        data_at Tsh tint (vint b) (Znth r reads); data_at Tsh tint (vint b) (Znth r lasts);
+        data_at Ews tint (vint b) (Znth r reads); data_at Ews tint (vint b) (Znth r lasts);
         comm_loc sh2 (Znth r locks) (Znth r comms) g g0 g1 g2 bufs sh gsh2 (map_upd h t (AE v0 Empty));
         data_at sh tbuffer (vint v) (Znth b bufs);
         ghost_var gsh1 (vint b) g0).
@@ -181,11 +181,11 @@ Definition finish_read_spec :=
   PRE [ _r OF tint ]
    PROP (readable_share sh)
    LOCAL (temp _r (vint r); gvars gv)
-   SEP (data_at sh (tarray (tptr tint) N) reads (gv _reading); data_at_ Tsh tint (Znth r reads))
+   SEP (data_at sh (tarray (tptr tint) N) reads (gv _reading); data_at_ Ews tint (Znth r reads))
   POST [ tvoid ]
    PROP ()
    LOCAL ()
-   SEP (data_at sh (tarray (tptr tint) N) reads (gv _reading); data_at Tsh tint Empty (Znth r reads)).
+   SEP (data_at sh (tarray (tptr tint) N) reads (gv _reading); data_at Ews tint Empty (Znth r reads)).
 
 Definition initialize_writer_spec :=
  DECLARE _initialize_writer
@@ -244,7 +244,7 @@ Definition finish_write_spec :=
   PRE [ ]
    PROP (0 <= b < B; 0 <= b0 < B; Forall (fun x => 0 <= x < B) lasts; Zlength h = N; Zlength shs = N;
          readable_share sh1; readable_share lsh; Forall readable_share shs;
-         sepalg_list.list_join sh0 shs Tsh; Forall isptr comms; b <> b0; ~In b lasts; ~In b0 lasts)
+         sepalg_list.list_join sh0 shs Ews; Forall isptr comms; b <> b0; ~In b lasts; ~In b0 lasts)
    LOCAL (gvars gv)
    SEP (data_at Ews tint (vint b) (gv _writing); data_at Ews tint (vint b0) (gv _last_given);
         data_at Ews (tarray tint N) (map (fun x => vint x) lasts) (gv _last_taken);
@@ -286,10 +286,10 @@ Definition reader_spec :=
    let '(r, reads, lasts, locks, comms, bufs, sh1, sh2, sh, g, g0, g1, g2, gv) := x in
    PROP (readable_share sh; readable_share sh1; readable_share sh2; isptr (Znth r comms))
    LOCAL (temp _arg arg; gvars gv)
-   SEP (data_at Tsh tint (vint r) arg; malloc_token Tsh tint arg;
+   SEP (data_at Ews tint (vint r) arg; malloc_token Tsh tint arg;
         data_at sh1 (tarray (tptr tint) N) reads (gv _reading); data_at sh1 (tarray (tptr tint) N) lasts (gv _last_read);
         data_at sh1 (tarray (tptr tint) N) comms (gv _comm); data_at sh1 (tarray (tptr tlock) N) locks (gv _lock);
-        data_at_ Tsh tint (Znth r reads); data_at_ Tsh tint (Znth r lasts);
+        data_at_ Ews tint (Znth r reads); data_at_ Ews tint (Znth r lasts);
         data_at sh1 (tarray (tptr tbuffer) B) bufs (gv _bufs);
         comm_loc sh2 (Znth r locks) (Znth r comms) g g0 g1 g2 bufs sh gsh2 empty_map;
         EX v : Z, data_at sh tbuffer (vint v) (Znth 1 bufs);
@@ -303,7 +303,7 @@ Definition writer_spec :=
   PRE [ _arg OF tptr tvoid ]
    let '(locks, comms, bufs, sh1, lsh, sh0, shs, g, g0, g1, g2, gv) := x in
    PROP (Zlength shs = N; readable_share sh1; readable_share lsh; Forall readable_share shs;
-         sepalg_list.list_join sh0 shs Tsh; Zlength g1 = N; Zlength g2 = N; Forall isptr comms)
+         sepalg_list.list_join sh0 shs Ews; Zlength g1 = N; Zlength g2 = N; Forall isptr comms)
    LOCAL (temp _arg arg; gvars gv)
    SEP (data_at_ Ews tint (gv _writing); data_at_ Ews tint (gv _last_given); data_at_ Ews (tarray tint N) (gv _last_taken);
         data_at sh1 (tarray (tptr tint) N) comms (gv _comm);
@@ -315,7 +315,7 @@ Definition writer_spec :=
         fold_right sepcon emp (map (ghost_var gsh1 (vint 0)) g1);
         fold_right sepcon emp (map (ghost_var gsh1 (vint 1)) g2);
         fold_right sepcon emp (map (fun i => EX sh : share,
-          !!(if eq_dec i 0 then sh = sh0 else if eq_dec i 1 then sh = sh0 else sh = Tsh) &&
+          !!(if eq_dec i 0 then sh = sh0 else if eq_dec i 1 then sh = sh0 else sh = Ews) &&
           EX v : Z, data_at sh tbuffer (vint v) (Znth i bufs)) (upto (Z.to_nat B))))
   POST [ tptr tvoid ] PROP () LOCAL () SEP ().
 
