sha/verif_SHA256.v
@@ -13,17 +13,17 @@ start_function.
 abbreviate_semax.
 
 forward_call (* SHA256_Init(&c); *)
-   (v_c).
+   (Tsh, v_c).
 rewrite !sepcon_assoc; (* need this with weak canceller *)
  apply sepcon_derives; [apply derives_refl | cancel].
 
 forward_call (* SHA256_Update(&c,d,n); *)
-  (@nil Z, data,v_c,d,dsh, Zlength data, gv).
+  (Tsh, @nil Z, data,v_c,d,dsh, Zlength data, gv).
  repeat split; auto; Omega1.
  simpl app.
 
 forward_call (* SHA256_Final(md,&c); *)
-    (sublist 0 (Zlength data) data, md, v_c, msh, gv).
+    (Tsh, sublist 0 (Zlength data) data, md, v_c, msh, gv).
 
 forward. (* return; *)
 change (Tstruct _SHA256state_st noattr) with t_struct_SHA256state_st.
