sha/verif_hmac_update.v
@@ -13,20 +13,22 @@ Require Import sha.hmac_common_lemmas.
 Require Import sha.hmac.
 Require Import sha.spec_hmac.
 
-Lemma updatebodyproof Espec c d len data gv (h1 : hmacabs)
-      (H : has_lengthD (s256a_len (absCtxt h1)) len data):
+Lemma updatebodyproof Espec wsh sh c d len data gv (h1 : hmacabs)
+      (H : has_lengthD (s256a_len (absCtxt h1)) len data)
+   (Hwsh: writable_share wsh)
+   (Hsh: readable_share sh):
 @semax CompSpecs Espec (func_tycontext f_HMAC_Update HmacVarSpecs HmacFunSpecs nil)
   (PROP  ()
    LOCAL  (temp _ctx c; temp _data d;
            temp _len (Vint (Int.repr len)); gvars gv)
-   SEP  (K_vector gv; hmacstate_ h1 c; data_block Tsh data d))
+   SEP  (K_vector gv; hmacstate_ wsh h1 c; data_block sh data d))
   (Ssequence (fn_body f_HMAC_Update) (Sreturn None))
   (frame_ret_assert
      (function_body_ret_assert tvoid
         (PROP  ()
          LOCAL ()
-         SEP  (K_vector gv; hmacstate_ (hmacUpdate data h1) c;
-         data_block Tsh data d))) emp).
+         SEP  (K_vector gv; hmacstate_ wsh (hmacUpdate data h1) c;
+         data_block sh data d))) emp).
 Proof. abbreviate_semax.
 unfold hmacstate_.
 Intros ST.
@@ -48,7 +50,7 @@ rewrite field_address_offset by auto with field_compatible.
 simpl @nested_field_type.
 make_Vptr c.
 simpl. rewrite Ptrofs.add_zero.
-Time forward_call (ctx, data, Vptr b i, d, Tsh, len, gv). (*6 versus 21 *)
+Time forward_call (wsh, ctx, data, Vptr b i, d, sh, len, gv). (*6 versus 21 *)
   { unfold sha256state_. Exists (fst ST).
     rewrite prop_true_andp by auto.
     change_compspecs CompSpecs.
@@ -71,7 +73,10 @@ destruct ST as [ST1 [ST2 ST3]]. simpl in *.
 Time cancel. (*0.5*)
 rewrite (field_at_data_at _ _ [StructField _md_ctx]).
 rewrite field_address_offset by auto with field_compatible.
-simpl. rewrite Ptrofs.add_zero. apply derives_refl. 
+simpl. 
+change (Tstruct _SHA256state_st noattr) with  t_struct_SHA256state_st.
+change_compspecs CompSpecs.
+rewrite Ptrofs.add_zero. apply derives_refl. 
 Time Qed. (*1.8*)
 
 Lemma body_hmac_update: semax_body HmacVarSpecs HmacFunSpecs
